---
tags:
  - mathematics/ordinary_differential_equations
---
# Exact Differential Equations

A differential expression $M(x, y)dx + N(x, y)dy$ is an exact differential in a region $R$ of the $xy$ plane if it corresponds to the differential of some function $f(x, y)$ defined in $R$. A first order ordinary differential equation of the form

$$
M(x, y)dx + N(x, y)dy = 0
$$

is said to be an exact equation if the expression on the left-hand side is an exact differential.

Criterion for an exact differential:
Let $M(x, y)$ and $N(x, y)$ be continuous and have continuous first partial derivatives in a rectangular region $R$ defined by $a < x < b, c < y < d$. Then a necessary and sufficient condition that $M(x, y)dx + N(x, y)dy$ be an exact differential is

$$
\frac{ \partial M }{ \partial y } = \frac{ \partial N }{ \partial x } 
$$

**Problem 1**

$$
\begin{align}
(2xy)dx + (x^{2} - 1)dy &= 0 \\
\frac{ \partial f }{ \partial x } &= 2xy \\
f(x, y) &= \int 2xy \ dx \\
f(x, y) &= 2y \int x \ dx \\
f(x, y) &= yx^{2} + g(y) \\
\frac{ \partial f }{ \partial y } &= x^{2} + g'(y) \\
x^{2} + g'(y) &= x^{2} - 1 \\
g'(y) &= -1 \\
g(y) &= -y \\
f(x, y) &= x^{2}y - y \\
x^{2}y - y &= C
\end{align}
$$

We can also solve it as a separable differential equation.

**Problem 2**

$$
\begin{align}
(e^{2y}- y \cos(xy)) dx + (2xe^{2y} - x \cos(xy)+ 2y)dy &= 0 \\
\frac{ \partial M }{ \partial y } = \frac{ \partial N }{ \partial x }  \to 2e^{2y} - (\cos(xy) - xy\sin(xy)) &= 2e^{2y} + xy \sin(xy) - \cos(xy) \\
\frac{ \partial f }{ \partial x }  &= e^{2y} - y \cos(xy) \\
f(x, y) &= \int e^{2y} - y \cos(xy) dx \\
f(x, y) &= e^{2y}x - \sin(xy) + g(y) \\
\frac{ \partial f }{ \partial y } &= 2e^{2y}x - x\cos(xy) + g'(y) \\
g'(y) + 2e^{2y}x - x \cos(xy) &= 2y + 2xe^{2y} - x \cos(xy) \\
g'(y) &= 2y \\
g(y) &= y^{2} \\
f(x, y) &= e^{2y}x - \sin(xy) + y^{2} \\
C &= e^{2y}x - \sin(xy) + y^{2} 
\end{align}
$$

**Problem 3**

Solve the initial value problem $\frac{dy}{dx} = \frac{xy^{2} - \cos x \sin x}{y(1-x^{2})}, \ y(0) = 2$

$$
\begin{align}
y(1-x^{2})dy &= (xy^{2} - \cos x \sin x) dx \\
y(x^{2} - 1)dy + (xy^{2} - \cos x \sin x) dx &= 0 \\
\frac{ \partial M }{ \partial y } &= 2x\mathbf{y}, \frac{ \partial N }{ \partial x } = 2xy \\
\frac{ \partial f }{ \partial y } &= y(x^{2} - 1) \\
f(x, y) &= \int y(x^{2} - 1) dy \\
f(x, y) &= \frac{1}{2}(x^{2} - 1)y^{2} + g(x) \\
f(x, y) &= \frac{1}{2}x^{2}y^{2} - \frac{1}{2}y^{2} + g(x) \\
\frac{ \partial f }{ \partial x } &= xy^{2} + g'(x) \\
xy^{2} + g'(x) &= xy^{2} - \cos x \sin x \\
g'(x) &= - \cos x \sin x \\
g'(x) &= -\frac{1}{2}\sin(2x) \\
g(x) &= -\frac{1}{2} \int \sin(2x) \ dx \\
g(x) &= \frac{1}{4} \cos (2x) \\
f(x, y) &= \frac{1}{2}(x^{2}-1)y^{2} + \frac{1}{4}\cos(2x) \\
C &= \frac{1}{2}(x^{2}-1)y^{2} + \frac{1}{4}\cos(2x) 
\end{align}
$$

Now, let $y(0) = 2$, then

$$
C = -\frac{7}{2}
$$

and therefore,

$$
2y^{2}(x^{2} - 1) + \cos(2x) = -7
$$
