---
tags:
  - mathematics/ordinary_differential_equations
---
# Homogenous Differential Equations with Constant Coefficients

We work with a second order differential equation with constant coefficients, which has the form

$$
ay'' + by' + cy = 0
$$

To solve any such equation, we first assume that $y = e^{rt}$ which means $y' = re^{rt}$ and $y'' = r^{2}e^{rt}$. Then, substituting this in to the equation above, we get

$$
\begin{align}
ar^{2}e^{rt} + bre^{rt} + ce^{rt} &= 0 \\
(ar^{2} + br + c)e^{rt} &= 0
\end{align}
$$

and since $e^{rt} \neq 0$ for any $r$, that means

$$
ar^{2} + br + c = 0
$$

which we can solve for $r$. This is called the **characteristic equation** for the differential equation, which tells us that if we find values $r$ that are solutions, then we immediately get that $y = e^{rt}$ is such a solution.

More specifically, let $y_{1}(t) = e^{r_{1}t}$ and $y_{2}(t) = e^{r_{2}t}$ which are two such solutions. Any linear combination of these two solutions also gives another solution, which we can define it as

$$
y = c_{1}y_{1}(t) + c_{2}y_{2}(t) = c_{1}e^{r_{1}t}+ c_{2}e^{r_{2}t}
$$

which is the set of all solutions. Differentiating and plugging this in to our original problem would show us that indeed every second order differential equation with constant coefficients has the solution form

$$
y = c_{1}e^{r_{1}t} + c_{2}e^{r_{2}t}
$$

**Problem 1**
Find the general solution of $y'' + 5' + 6y = 0$.

$$
\begin{align}
y'' + 5y' + 6y &= 0 \\
r^{2} + 5r + 6 &= 0 \\
(r+3)(r+2) &= 0 \\
r &= -3, -2 \\
y &= C_{1}e^{-2t} + C_{2}e^{-3t}
\end{align}
$$

**Problem 2**
Find the solution of the initial value problem $4y'' - 8y' + 3y = 0, \quad y(0) = 2, \  y'(0) = \frac{1}{2}$

$$
\begin{align}
4y'' - 8y' + 3y &= 0 \\
4r^{2} - 8r + 3 &= 0 \\
(2r - 1)(2r - 3) &= 0 \\
r &= \frac{1}{2}, \frac{3}{2} \\
y &= C_{1}e^{1/2t} + C_{2}e^{3/2t} \\
 & \begin{cases}
C_{1} + C_{2} = 2 \\
\frac{3}{2}C_{2} + \frac{1}{2}C_{1} = \frac{1}{2}
\end{cases} \\
c_{2} &= -\frac{1}{2}, \  c_{1} = \frac{5}{2} \\
y &= -\frac{1}{2}e^{3t/2} + \frac{5}{2}e^{t/2}
\end{align}
$$