---
tags:
  - mathematics/ordinary_differential_equations
---
# Repeated Roots

In earlier sections we showed how to solve the equation

$$
ay'' + by' + cy = 0
$$

when the roots of the characteristic equation

$$
ar^{2} + br + c = 0
$$

either are real and different or are complex conjugates. Now we consider the third possibility, namely, that the roots $r_{1}$ and $r_{2}$ are equal. This case is transitional between the other two and occurs when the discriminant $b^{2} - 4ac$ is zero. Then it follows from the quadratic formula that

$$
r_{1} = r_{2} = -\frac{b}{2a}
$$

The difficulty is immediately apparent, both roots yield the same solution

$$
y_{1}(t) = e^{-bt/2a}
$$

of the differential equation, and it is not obvious how to find a second solution. One method we can find this second solution comes from D'Alembert, whereby we normally have one solution be $cy_{1}(t)$, so now lets find some function $v(t)$ where $v(t)y_{1}(t)$ is the solution. Let's try it for the equation ${} y'' + 4y' + 4y = 0 {}$.

$$
y = v(t)y_{1}(t) = v(t)e^{-2t}
$$

we have

$$
y' = v'(t)e^{-2t} - 2v(t)e^{-2t}
$$

and

$$
y'' = v''(t)e^{-2t} - 4v'(t)e^{-2t} + 4v(t)e^{-2t}
$$

then substituting all these into our original equation at the top, we get

$$
[v''(t) - 4v'(t) + 4v(t) + 4v'(t) - 8v(t) + 4v(t)]e^{-2t} = 0
$$

which simplifies down to $v''(t) = 0$ and hence $v'(t) = c_{1}$ which finally implies $v(t) = c_{1}t + c_{2}$. Therefore, now that we found $v(t)$ lets plug it back at the top to get

$$
y = c_{1}te^{-2t} + c_{2}e^{-2t}
$$

which gives us our solution. We can compute the Wronskian and see that indeed the two solutions are independent and hence form the fundamental set of solutions.

This can be generalized, and we find that if $r_{1} = r_{2}$ then the general solution turns out to become,

$$
y = c_{1}e^{r_{1}t} + c_{2}te^{r_{1}t}
$$

**Problem 1**
Solve the following ordinary differential equation, $y'' - 10y' + 25y = 0$

$$
\begin{align}
y'' - 10y' + 25y &= 0 \\
r^{2} - 10r + 25 &= 0 \\
(r-5)^{2} &= 0 \\
r &= 5 \\
y &= C_{1}e^{5t} + C_{2}te^{5t}
\end{align}
$$