---
tags:
  - mathematics/ordinary_differential_equations
---
# Nonhomogeneous Equations, Method of Undetermined Coefficients

> [!theorem] **Theorem**
> If $Y_{1}$ and $Y_{2}$ are two solutions of the nonhomogeneous equation $y'' + p(t)y' + q(t)y = g(t)$, then their difference $Y_{1} - Y_{2}$ is a solution of the corresponding homogeneous equation $y'' + p(t)y' + q(t)y = 0$. If, in addition, $y_{1}$ and $y_{2}$ are a fundamental set of solutions, then
>
> $$
> Y_{1}(t) - Y_{2}(t) = c_{1}y_{1}(t) + c_{2}y_{2}(t)
> $$
>
> where $c_{1}$ and $c_{2}$ are certain constants.

*Proof*

To prove this result, we first define $L[y]$.

$L[y] = y'' + p(t)y' + q(t)y = g(t)$

Note that $Y_{1}$ and $Y_{2}$ satisfy the equations

$$
L[Y_{1}](t) = g(t), \quad L[Y_{2}](t) = g(t)
$$

and therefore,

$$
L[Y_{1}](t) - L[Y_{2}](t) = g(t) - g(t) = 0
$$

However,

$$
L[Y_{1}] - L[Y_{2}] = L[Y_{1} - Y_{2}]
$$

so this means,

$$
L[Y_{1} - Y_{2}](t) = 0
$$

and so $Y_{1} - Y_{2}$ is also a valid solution to our equation. Since all solutions can be expressed as a linear combinations of a fundamental set of solutions, it means $Y_{1} - Y_{2}$ can also be written as a fundamental set of solutions and the theorem holds.

$$
\tag*{\(\blacksquare\)}
$$

> [!theorem] **Theorem**
> The general solution of the nonhomogeneous equation $y'' + p(t)y' + q(t)y = g(t)$ can be written in the form
>
> $$
> y = \phi(t) = c_{1}y_{1}(t) + c_{2}y_{2}(t) + Y(t)
> $$
>
> where $y_{1}$ and $y_{2}$ are a fundamental set of solutions of the corresponding homogenous equation $y'' + p(t)y' + q(t)y = 0$, $c_{1}$ and $c_{2}$ are arbitrary constants, and $Y$ is some specific solution of the nonhomogeneous equation.

*Proof*

Let $\phi(t)$ be an arbitrary solution we can identify as $Y_{1}$ and also let $Y$ denote the solution of $Y_{2}$, then using our previous theorem we have

$$
\phi(t) - Y(t) = c_{1}y_{1}(t) + c_{2}y_{2}(t)
$$

which thus gives us the equation in the theorem since $\phi$ is arbitrary. Therefore, we can refer to $\phi$ as the general solution now of the nonhomogeneous equation.

$$
\tag*{\(\blacksquare\)}
$$

> [!example] **Example** (Example 1)
> Find a particular solution of
>
> $$
> y'' - 3y' - 4y = 3e^{2t}
> $$
>
> We seek a function $Y$ such that the combination $Y''(t) - 3Y'(t) - 4Y(t)$ is equal to $3e^{2t}$. Since the exponential function reproduces itself through differentiation, the most plausible way to achieve the desired result is to assume that $Y(t)$ is some multiple of $e^{2t}$.
>
> $$
> Y(t) = Ae^{2t}
> $$
>
> where the coefficient $A$ is yet to be determined. To find $A$, we calculate
>
> $$
> Y'(t) = 2Ae^{2t}, \quad Y''(t) = 4Ae^{2t}
> $$
>
> and substitute for $y, y',$ and $y''$ we obtain
>
> $$
> (4A - 6A - 4A)e^{2t} = 3e^{2t}
> $$
>
> Hence $-6Ae^{2t}$ must equal $3e^{2t}$, so $A = -1/2$. Thus a particular solution is
>
> $$
> Y(t) = -\frac{1}{2}e^{2t}
> $$

> [!example] **Example** (Example 2)
> Find a particular solution of
>
> $$
> y'' - 3y' - 4y = 2 \sin t
> $$
>
> We use the assumption that our solution takes the form
>
> $$
> Y(t) = A \sin t + B \cos t
> $$
>
> where $A$ and $B$ are to be determined. Then
>
> $$
> Y'(t) = A \cos t - B \sin t, \quad Y''(t) = - A \sin t - B \cos t
> $$
>
> By substituting these expressions for $y, y',$ and $y''$ and collecting terms we get
>
> $$
> (-A + 3B - 4A) \sin t + (-B - 3A -4B) \cos t = 2 \sin t
> $$
>
> And so in order to match the coefficients, we need to satisfy the following system of equations
>
> $$
> -5A + 3B = 2, \quad -3A - 5B = 0
> $$
>
> By solving this system of equations, we obtain $A = -\frac{5}{17}$ and $B = \frac{3}{17}$ hence a particular solution is
>
> $$
> Y(t) = -\frac{5}{17} \sin t + \frac{3}{17} \cos t
> $$

> [!example] **Example** (Example 3)
> Find a particular solution of
>
> $$
> y'' - 3y' - 4y = -8e^{t} \cos 2 t
> $$
>
> In this case we assume that $Y(t)$ is the product of $e^{t}$ and a linear combination of $\cos 2t$ and $\sin 2t$; that is
>
> $$
> Y(t) = Ae^{t} \cos 2t + B e^{t} \sin 2t
> $$
>
> It follows that,
>
> $$
> Y'(t) = (A + 2B)e^{t} \cos 2t + (-2A + B)e^{t} \sin 2t
> $$
>
> and
>
> $$
> Y''(t) = (-3A + 4B)e^{t} \cos 2t + (-4A - 3B)e^{t} \sin 2t.
> $$
>
> By substituting these equations, we need to find $A$ and $B$ that satisfy
>
> $$
> 10A + 2B = 8, \quad 2A - 10B = 0
> $$
>
> Hence, $A = \frac{10}{13}$ and $B = \frac{2}{13}$ therefore, a particular solution is
>
> $$
> Y(t) = \frac{10}{13}e^{t} \cos 2t + \frac{2}{13} e^{t} \sin 2t
> $$

> [!example] **Example** (Example 4)
> Find a particular solution of
>
> $$
> y'' - 3y' - 4y = 3e^{t} + 2\sin t - 8e^{t} \cos 2t
> $$
>
> which when we split up the equation, we get three other equations.
>
> $$
> \begin{align}
> y'' - 3y' - 4y &= 3e^{2t} \\
> y'' - 3y' - 4y &= 2 \sin t \\
> y'' - 3y' - 4y &= -8e^{t} \cos 2t
> \end{align}
> $$
>
> Solutions of these three equations were found in the above three examples, and hence the solution is just their sum which is
>
> $$
> Y(t) = -\frac{1}{2}e^{2t} + \frac{3}{17}\cos t - \frac{5}{17} \sin t + \frac{10}{13} e^{t} \cos 2t + \frac{2}{13} e^{t} \sin 2t
> $$