---
tags:
  - mathematics/ordinary_differential_equations
---
# Higher order Homogeneous Equations with Constant Coefficients

> [!problem] **Problem** (Problem 1)
> Find the general solution of
>
> $$
> y^{(4)} + y''' - 7y'' - y' + 6y = 0
> $$
>
> The characteristic equation of the ordinary differential equation is the following,
>
> $$
> r^{4} + r^{3} - 7r^{2} - r + 6 = 0
> $$
>
> To find roots, we test out some numbers and then do polynomial long division to simplify further. We use the rational root theorem to get numbers to test out, those being $\pm 1, \pm 2, \pm 3, \pm 6$. Let us try $r = 1$, and we get that it indeed is a solution. Then, doing long division we get
>
> $$
> \begin{align}
> \begin{array}{r|rrrrr} 1 & 1 & 1 & -7 & -1 & 6 \\ & & 1 & 2 & -5 & -6 \\ \hline & 1 & 2 & -5 & -6 & 0 \\ \end{array}
>  \\ \\
> (r - 1)(r^{3} - 2r^{2} - 5r - 6)
> \end{align}
> $$
>
> Using the rational root theorem again, we get $r = -1$, and doing polynomial long division again we have
>
> $$
> \begin{align}
> \begin{array}{r|rrrr} -1 & 1 & 2 & -5 & -6 \\ & & -1 & -1 & 6 \\ \hline & 1 & 1 & -6 & 0 \\ \end{array} \\ \\
> (r-1)(r+1)(r^{2} + r - 6)
> \end{align}
> $$
>
> Finally we factor, getting
>
> $$
> (r-1)(r+1)(r+3)(r-2)
> $$
>
> which means $r = 1, -1, -3, 2$. Thus our general solution is,
>
> $$
> y_{c} = C_{1}e^{t} + C_{2}e^{-t} + C_{3}e^{-3t} + C_{4}e^{2t}
> $$

> [!problem] **Problem** (Problem 2)
> Find the general solution of
>
> $$
> y^{(4)} + 2y'' + y = 0
> $$
>
> The characteristic equation of the differential equation is,
>
> $$
> r^{4} + 2r^{2} + 1 = 0
> $$
>
> which when factored gives us
>
> $$
> (r^{2}+1)(r^{2}+1) = 0
> $$
>
> implicating that we have the solutions $r_{1} = r_{2} = i$ and $r_{3} = r_{4} = -i$. All that remains is to write the general solution, which is
>
> $$
> y_{c} = C_{1}\sin(t) + C_{2}\cos(t) + C_{3}t\sin(t) + C_{4}t\cos(t)
> $$
