---
tags:
  - mathematics/ordinary_differential_equations
---
# Method of Undetermined Coefficients for Higher order Differential Equations

> [!example] **Example** (Example 1)
> Find the general solution of
>
> $$
> y''' - 3y'' + 3y' - y = 4e^{t}
> $$
>
> The characteristic polynomial for the homogeneous equation is
>
> $$
> r^{3} - 3r^{2} + 3r - 1 = (r-1)^{3},
> $$
>
> so the general solution of the homogeneous equation is
>
> $$
> y_{c}(t) = c_{1}e^{t} + c_{2}te^{t} + c_{3}t^{2}e^{t}
> $$
>
> To find a particular solution $Y(t)$, we first assume that $Y(t) = Ae^{t}$ but the issue is that we have multiples of $t$. So we need to multiply this by $t^{3}$ instead, so our assumption would end up being $Y(t) = At^{3}e^{t}$, where $A$ is an undetermined coefficient. Differentiate $Y(t)$ three times, substitute for $y$ and its derivatives and we get
>
> $$
> 6Ae^{t} = 4e^{t}
> $$
>
> Thus $A = \frac{2}{3}$ and the particular solution is
>
> $$
> Y(t) = \frac{2}{3}t^{3}e^{t}
> $$
>
> The general solution is the sum of $y_{c}(t)$ and $Y(t)$, which is
>
> $$
> y = c_{1}e^{t} + c_{2}te^{t} + c_{3}t^{2}e^{t} + \frac{2}{3}t^{3}e^{t}
> $$

> [!example] **Example** (Example 2)
> Find a particular solution of the equation
>
> $$
> y^{(4)} + 2y'' + y = 3 \sin t - 5 \cos t
> $$
>
> The general solution of the homogeneous equation is
>
> $$
> y_{c}(t) = c_{1}\cos t + c_{2} \sin t + c_{2} t \cos t + c_{4} t \sin t
> $$
>
> corresponding to the roots $r = i, i, -i, -i$ of the characteristic equation. Our initial assumption for a particular solution is $Y(t) = A \sin t + B \cos t$, but we must multiply this choice by $t^{2}$ to make it different from all solutions of the homogeneous equation. Thus our final assumption is
>
> $$
> Y(t) = A t^{2} \sin t + B t^{2} \cos t
> $$
>
> Next, we differentiate $Y(t)$ four times, substitute into the differential equation, and collect terms, obtaining finally
>
> $$
> -8 A \sin t - 8 B \cos t = 3 \sin t - 5 \cos t
> $$
>
> Thus $A = -\frac{3}{8}, B = \frac{5}{8}$ and the particular solution is
>
> $$
> Y(t) = -\frac{3}{8}t^{2} \sin t + \frac{5}{8} t^{2} \cos t
> $$

> [!example] **Example** (Example 3)
> Find a particular solution of
>
> $$
> y''' - 4y' = t + 3 \cos t + e^{-2t}
> $$
>
> First we solve the homogeneous equation.  The characteristic equation is $r^{3} - 4r = 0$ and the roots are $r = 0, \pm 2$ hence
>
> $$
> y_{c}(t) = C_{1} + C_{2}e^{2t} + C_{3}e^{-2t}
> $$
>
> We can write a particular solution as the sum of the particular solutions of the differential equations
>
> $$
> \begin{align}
> y''' - 4y' &= t \\
> y''' - 4y' &= 3 \cos t \\
> y''' - 4y'&= e^{-2t}
> \end{align}
> $$
>
> Our initial choice for a particular solution $Y_{1}(t)$ of the first equation is $A_{0}t + A_{1}$, but a constant is a solution of the homogeneous equation, so we multiply by $t$. Thus
>
> $$
> Y_{1}(t) = t(A_{0}t + A_{1})
> $$
>
> For the second equation we choose
>
> $$
> Y_{2}(t) = B \cos t + C \sin t
> $$
>
> and there is no need to modify this initial choice since $\sin t$ and $\cos t$ are not solutions of the homogeneous equation. Finally, for the third equation, since $e^{-2t}$ is a solution of the homogeneous equation, we assume that
>
> $$
> Y_{3}(t) = Ete^{-2t}
> $$
>
> The constants are determined by substituting into the individual differential equations; they are $A_{0} = -\frac{1}{8}, A_{1} = 0, B = 0, C = -\frac{3}{5}, E = \frac{1}{8}$. Hence a particular solution
>
> $$
> Y(t) = -\frac{1}{8}t^{2} - \frac{3}{5} \sin t + \frac{1}{8} t e^{-2t}
> $$
