---
tags:
  - mathematics/ordinary_differential_equations
---
# The Laplace Transform

> [!definition] **Definition** (Laplace Transform)
> Let $f$ be a function defined for $t \geq 0$. Then the integral
>
> $$
> L\{ f(t) \} = \int_{0}^{\infty} e^{-st}f(t)dt = F(s)
> $$
>
> is said to be the Laplace transform of $f$, provided that the integral converges.

> [!example] **Example** (Evaluate ${} L\{ 1 \} {}$)
> Evaluate $L\{ 1 \}$
>
> $$
> \begin{align}
> L\{ 1 \} &= \int_{0}^{\infty} e^{-st}(1)dt \\
> &= \lim_{ b \to \infty} \int^{b}_{0}e^{-st}dt \\
> &= \lim_{b \to \infty} \left[ - \frac{1}{s} e^{-st}  \right]_{0}^{b} \\
> &= -\frac{1}{s}[\lim_{b \to \infty} e^{-st} - 1] \\
> &= \frac{1}{s}
> \end{align}
> $$

> [!example] **Example** (Evaluate ${} L\{ t \} {}$)
> Evaluate $L\{ t \}$
>
> $$
> \begin{align}
> L\{ t \} &= \int_{0}^{\infty} e^{-st}t \ dt \\
> &= \left[ -\frac{1}{s}te^{-st} - \frac{1}{s^{2}}e^{-st} \right]_{0}^{\infty} \\
> &= (0-0) - \left( 0 - \frac{1}{s ^{2}} \right) \\
> &= \frac{1}{s ^{2}}
> \end{align}
> $$

> [!example] **Example** (Evaluate $L\{ e^{-3t} \}$)
> Evaluate $L\{ e^{-3t} \}$
>
> $$
> \begin{align}
> L\{ e^{-3t} \} &= \int_{0}^{\infty} e^{-st}e^{-3t}dt \\
> &= \int_{0}^{\infty} e^{-(s+3)t} dt \\
> &= \left[ \frac{1}{-(s+3)}e^{-(s+3)t} \right]_{0}^{\infty} \\
> &= 0 - \left( - \frac{1}{s+3} \cdot  1 \right) \\
> &= \frac{1}{s+3}
> \end{align}
> $$

> [!example] **Example** (Evaluate ${} L\{ \sin 2t \} {}$)
> Evaluate $L\{ \sin 2t \}$
>
> $$
> \begin{align}
> L\{ \sin(2t) \} &= \int_{0}^{\infty} e^{-st}\sin(2t)dt \\
> &= \frac{2}{s^{2} + 4}
> \end{align}
> $$

The Laplace transform is linear,

$$
L\{ af(t) + bg(t) \} = a L\{ f(t) \} + b L \{ g(t) \}
$$

> [!example] **Example** (Evaluate More Laplace Transforms)
> Now use the Laplace transform formulas to find the following Laplace transforms:
>
> $$
> \begin{align}
> L\{ 1 + 5t \} &= \frac{1}{s} + \frac{5}{s^{2}} \\
> L\{ 4e^{5t} - 10 \sin 2t \} &= \frac{4}{s-5} - \frac{10}{s^{2} + 4} \\
> L\{ 20e^{-3t} + 7t - 9 \} &= \frac{20}{s+3} + \frac{7}{s^{2}} - \frac{9}{s}
> \end{align}
> $$
>
> Use the Laplace transform to find $L\{ f(t) \}$ where
>
> $$
> f(t) = \begin{cases}
> 0, & 0 \leq t < 3 \\
> 2, & t \geq 3
> \end{cases}
> $$
>
> Note that $L\{2 \} = \int_{3}^{\infty} e^{-st}(2)dt = -\frac{2}{s} \cdot \frac{1}{e^{st}} |_{3}^{\infty}$. Which is just $F(s) = \frac{2e^{-3s}}{s}$,
>
> $$
> L\{ f(t) \} = \begin{cases}
> 0,  & 0 \leq t < 3 \\
> \frac{2}{s}e^{-3s},  & t \geq 3
> \end{cases}
> $$

> [!example] **Example** (Finding the Laplace Transform with $e^{t}$ function product)
> Evaluate $L\{ te^{3t} \}$
>
> $$
> \begin{align} \\
> L\{ te^{3t} \} &= L\{ t \}|_{s \to s-3} \\
> L\{ t \}|_{s \to s - 3} &= \frac{1}{s^{2}}|_{s \to s-3} \\
> &= \frac{1}{(s-3)^{2}}
> \end{align}
> $$