---
tags:
  - mathematics/ordinary_differential_equations
---
# Solutions of Initial Value Problems

> [!definition] **Definition** (Inverse Laplace Transform)
> If $F(s)$ represents the Laplace Transform of $f(t)$, we say $f(t)$ is the inverse Laplace transform of $F(s)$ and we write $L^{-1}\{ F(s) \} = f(t)$.

## Inverse Laplace Transforms

Now evaluate the following inverse Laplace transforms,
**Problem 1**

$$
\begin{align}
L^{-1}\left\{  \frac{1}{s ^{5}}  \right\} &= \frac{1}{4!} L^{-1}\left\{  \frac{4!}{s^{5}}  \right\} \\
&= \frac{1}{24} t^{4}
\end{align}
$$

**Problem 2**

$$
\begin{align}
L ^{-1} \left\{  \frac{1}{s^{2} + 7}  \right\} = \frac{1}{\sqrt{7}} L ^{-1} \left\{  \frac{\sqrt{7}}{s^{2} + 7}  \right\} \\
\frac{1}{\sqrt{7}} \sin(\sqrt{7}t)
\end{align}
$$

**Problem 3**

$$
\begin{align}
L ^{-1} \left\{  \frac{-2s+6 }{s ^{2} + 4} \right\} &= -2L ^{-1}\left\{  \frac{s}{s^{2} + 4}  \right\} + 3L ^{-1} \left\{ \frac{2}{s^{2} + 4}  \right\} \\
&= -2\cos(2t) + 3\sin(2t)
\end{align}
$$

**Problem 4**

$$
\begin{align}
 & L ^{-1}\left\{  \frac{x^{2} + 6s + 9}{(s-1)(s-2)(s+4)}  \right\} \\
\frac{s^{2} + 6s + 9}{(s-1)(s-2)(s+4)} &= \frac{A}{s-1} + \frac{B}{s-2} + \frac{C}{s+4} \\
s ^{2} + 6s + 9 &= A(s-2)(s+4) + B(s-1)(s+4) + C(s-1)(s-2) \\
\text{Let } s &= 2, \\
25 &= 6B \to B = \frac{25}{6} \\
\text{Let } s &= 1, \\
16 &= -5A \to A = -\frac{16}{5} \\
\text{Let } s &= -4, \\
16-24 + 9 &= -30C \to C = \frac{1}{30} \\
&= -\frac{16}{5}L ^{-1} \left\{  \frac{1}{s-1}  \right\} + \frac{25}{6}L ^{-1} \left\{  \frac{1}{s-2}  \right\} + \frac{1}{30}L ^{-1} \left\{  \frac{1}{s+4}  \right\} \\
&=-\frac{16}{5}e^{t} + \frac{25}{6}e^{2t} + \frac{1}{30}e^{-4t}
\end{align}
$$

**Problem 5**

$$
\begin{align}
L ^{-1} \left\{  \frac{2s + 5}{(s-3)^{2}}  \right\} \\
\frac{2s + 5}{(s-3)^{2}} &= \frac{A}{s-3} + \frac{B}{(s-3)^{2}} \\
2s + 5 &= A(s-3) + B \\
2s + 5 &= As + (-3A + B) \\
A &= 2, \\
5 &= -3A + B \to 5 = -6 + B \to B = 11 \\
L ^{-1} \left\{  \frac{2s + 5}{(s-3)^{2}}  \right\} &= 2L^{-1} \left\{  \frac{1}{s-3}  \right\} + 11 L ^{-1}\left\{  \frac{1}{(s-3)^{2}}  \right\} \\
&= 2e^{3t} + 11te^{3t}
\end{align}
$$

## Initial Value Problems with Laplace Transforms

**Problem 1**

$$
\begin{align}
\frac{dy}{dt} + 3y &= 13 \sin 2t, \quad y(0) = 6 \\
L\left\{  \frac{dy}{dt}  \right\} + 3L\{ y \} &= 13L\{ \sin 2t \} \\
sY(s) - y(0) + 3Y(s)&= 13 \cdot  \frac{2}{s^{2} + 4} \\
sY(s) +3Y(s) - 6 &= \frac{26}{s^{2} + 4} \\
Y(s)(s+3) &= \frac{26}{s^{2} + 4} + \frac{6(s^{2} + 4)}{s^{2} + 4} \\
Y(s) &= \frac{26 + 6s^{2} + 24}{(s^{2} + 4)(s+3)} \\
Y(s) &= \frac{6s^{2} + 50}{(s^{2} + 4)(s+3)}
\end{align}
$$

Now we do partial fraction decomposition,

$$
\begin{align}
\frac{6s^{2} + 50}{(s^{2} + 4)(s+3)} &= \frac{A}{s+3} + \frac{Bs + C}{s^{2} + 4} \\
6s^{2} + 50 &= A(s^{2} +4) + (Bs + C)(s+3) \\
\text{Let } s= -3, \\
104 &= 13A \to A = 8 \\
6s^{2} + 50 &= As^{2} + 4A + Bs^{2} + 3Bs + Cs + 3C \\
6s^{2} + 50 &= s^{2}(A + B) + s(3B + C ) + (4A + 3C) \\
6 &= A + B \to B = -2 \\
50 &= 4A + 3C \to C = 6 \\
\frac{6s^{2} + 50}{(s^{2} + 4)(s+3)} &= \frac{8}{s+3} + \frac{-2s + 6}{s^{2} + 4}
\end{align}
$$

And finally apply the inverse Laplace transform,

$$
\begin{align}
Y(s) &= \frac{8}{s+3} + \frac{-2s + 6}{s^{2} + 4} \\
Y(s) &= \frac{8}{s+3} + \frac{-2s}{s^{2} + 4}  + \frac{6}{s^{2} + 4} \\
L ^{-1}(Y(s)) &= 8 L ^{-1}\left\{  \frac{1}{s+3}  \right\} -2 L ^{-1}\left\{  \frac{s}{s^{2} +4}  \right\} + 3 L ^{-1} \left\{  \frac{2}{s^{2} + 4}  \right\}\\
y(t) &= 8e^{-3t} -2\cos(2t) + 3 \sin(2t)
\end{align}
$$
