---
tags:
  - mathematics/ordinary_differential_equations
---
# Step Functions

> [!definition] **Definition** (Unit Step Function)
> A unit step function $u(t-a)$ is defined to be
>
> $$
> u(t-a) = \begin{cases}
> 0 & 0 \leq t < a \\
> 1 & t \geq a
> \end{cases}
> $$

The piecewise-defined function

$$
f(t) = \begin{cases}
g(t), & t < a \\
h(t),  & t \geq a
\end{cases}
$$

can be rewritten using unit step functions as $f(t) = g(t) - g(t)u(t-a) + h(t)u(t-a)$.

> [!definition] **Definition** (Rectangular Window Function)
> The rectangular window function is defined by
>
> $$
> \Pi_{a, b} (t) = u(t-a)-u(t-b) = \begin{cases}
> 0, & t<a \\
> 1, & a\leq t\leq b \\
> 0, & t>b
> \end{cases}
> $$
>
> and in terms of unit step functions as $g(t)[u(t-a) - u(t-b)]$.

> [!problem] **Problem** (Problem 1)
> Express $f(t) = \begin{cases}20t,  & t < 5 \\0,  & t \geq 5\end{cases}$ in terms of unit step functions.
>
> $$
> f(t) = 20t - 20tu(t-5)
> $$

> [!theorem] **Theorem** (Laplace Transforms of Step Functions)
> Note that,
>
> $$
> L\{ u(t-a) \} = \frac{e^{-as}}{s}
> $$
>
> and more generally that
>
> $$
> L\{ f(t-a)u(t-a) \} = e^{-as}F(s) = e^{-as}L^{-1}\{ f(t) \}
> $$

> [!problem] **Problem** (Problem 2)
> Find the Laplace transform of $f(t) = 2 - 3u(t-2) + u(t-3)$.
>
> $$
> \begin{align}
> f(t) &= 2 - 3u(t-2) + u(t-3) \\
> f(t) &= 2 - 3u_{2}(t) + u_{3}(t) \\
> F(s) &= \frac{2}{s} - \frac{3e^{-2s}}{s} + \frac{e^{-3s}}{s}
> \end{align}
> $$

> [!problem] **Problem** (Problem 3)
> The function of $f$ is defined as
>
> $$
> f(t) = \begin{cases}
> \sin t,  & 0\leq t \leq \frac{\pi}{4} \\
> \sin t + \cos\left( t-\frac{\pi}{4} \right),  & t \geq \frac{\pi}{4}
> \end{cases}
> $$
>
> now find $L\{ f(t) \}$.
>
> $$
> \begin{align}
> f(t) &= \sin(t) + \cos\left( t - \frac{\pi}{4} \right)u_{\frac{\pi}{4}}(t) \\
> F(s) &= L\{ \sin(t) \} + L\left\{  \cos\left( t-\frac{\pi}{4} \right) u_{\frac{\pi}{4}}(t) \right\} \\
> &= \frac{1}{s^{2} + 1} + \frac{e^{\pi/4}s}{s^{2} + 1} \\
> &= \frac{1 + se^{-\pi/4}}{s^{2} + 1}
> \end{align}
> $$

> [!problem] **Problem** (Problem 4)
> Find the inverse transform of
>
> $$
> F(s) = \frac{1 - e^{-2s}}{s^{2}}
> $$
>
> From linearity we get
>
> $$
> \begin{align}
> f(t) &= L ^{-1} \{ F(s) \}  \\
> &= L ^{-1} \left\{   \frac{1}{s^{2}}  \right\} - L ^{-1} \left\{  \frac{e^{-2s}}{s^{2}}  \right\} \\
> &= t - u_{2}(t)(t-2)
> \end{align}
> $$
>
> which is simply
>
> $$
> f(t) = \begin{cases}
> t,  & 0 \leq t < 2 \\
> 2, & t \geq 2
> \end{cases}
> $$

> [!problem] **Problem** (Problem 5)
> Find the inverse transform of
>
> $$
> G(s) = \frac{1}{s^{2} - 4s + 5}
> $$
>
> We complete the square,
>
> $$
> G(s) = \frac{1}{(s-2)^{2} + 1} = F(s-2)
> $$
>
> where $F(s) = (s^{2} + 1)^{-1}$. Since $L ^{-1} \{ F(s) \} = \sin t$, it follows that
>
> $$
> g(t) = L ^{-1} \{  G(s) \} = e^{2t} \sin t
> $$
