---
tags:
  - mathematics/ordinary_differential_equations
---
# Systems of Equations, Eigenvalues, Eigenvectors

## Example 1: Solving a System of Linear Equations

We are given the following system of linear equations:

$$
\begin{align}
x_1 - 2x_2 + 3x_3 &= 7 \\
-x_1 + x_2 - 2x_3 &= -5 \\
2x_1 - x_2 - x_3 &= 4
\end{align}
$$

The augmented matrix corresponding to this system is:

$$
\left(\begin{array}{ccc|c}
1 & -2 & 3 & 7 \\
-1 & 1 & -2 & -5 \\
2 & -1 & -1 & 4
\end{array}\right)
$$

### Step 1: Row Operations

#### (a) Add the First Row to the Second Row and Add \(-2\) times the First Row to the Third Row.

We perform the following row operations:

$$
R_2 \to R_2 + R_1, \quad R_3 \to R_3 - 2R_1
$$

Resulting matrix:

$$
\left(\begin{array}{ccc|c}
1 & -2 & 3 & 7 \\
0 & -1 & 1 & 2 \\
0 & 3 & -7 & -10
\end{array}\right)
$$

#### (b) Multiply the Second Row by \(-1\).

$$
R_2 \to -R_2
$$

Resulting matrix:

$$
\left(\begin{array}{ccc|c}
1 & -2 & 3 & 7 \\
0 & 1 & -1 & -2 \\
0 & 3 & -7 & -10
\end{array}\right)
$$

#### (c) Add \(-3\) times the Second Row to the Third Row.

$$
R_3 \to R_3 - 3R_2
$$

Resulting matrix:

$$
\left(\begin{array}{ccc|c}
1 & -2 & 3 & 7 \\
0 & 1 & -1 & -2 \\
0 & 0 & -4 & -4
\end{array}\right)
$$

#### (d) Divide the Third Row by \(-4\).

$$
R_3 \to \frac{1}{-4} R_3
$$

Resulting matrix:

$$
\left(\begin{array}{ccc|c}
1 & -2 & 3 & 7 \\
0 & 1 & -1 & -2 \\
0 & 0 & 1 & 1
\end{array}\right)
$$

Now, the system corresponds to the following triangular system of equations:

$$
\begin{align}
x_1 - 2x_2 + 3x_3 &= 7 \\
x_2 - x_3 &= -2 \\
x_3 &= 1
\end{align}
$$

### Step 2: back Substitution

From the third equation, we already know that:

$$
x_3 = 1
$$

Substitute $x_3 = 1$ into the second equation:

$$
x_2 - 1 = -2 \quad \Rightarrow \quad x_2 = -1
$$

Finally, substitute $x_2 = -1$ and $x_3 = 1$ into the first equation:

$$
x_1 - 2(-1) + 3(1) = 7 \quad \Rightarrow \quad x_1 + 2 + 3 = 7 \quad \Rightarrow \quad x_1 = 2
$$

Thus, the solution to the system is:

$$
\mathbf{x} = \begin{pmatrix} 2 \\ -1 \\ 1 \end{pmatrix}
$$

Since the solution is unique, we conclude that the coefficient matrix is nonsingular.

## Example 2: Solutions to a Parametric System

Consider the system:

$$
\begin{align}
x_1 - 2x_2 + 3x_3 = b_1 \\
-x_1 + x_2 - 2x_3 = b_2 \\
2x_1 - x_2 + 3x_3 = b_3
\end{align}
$$

The augmented matrix for this system is:

$$
\left(\begin{array}{ccc|c}
1 & -2 & 3 & b_1 \\
-1 & 1 & -2 & b_2 \\
2 & -1 & 3 & b_3
\end{array}\right)
$$

### Step 1: Row Operations

#### (a) Add the First Row to the Second Row and Add \(-2\) times the First Row to the Third Row.

$$
R_2 \to R_2 + R_1, \quad R_3 \to R_3 - 2R_1
$$

Resulting matrix:

$$
\left(\begin{array}{ccc|c}
1 & -2 & 3 & b_1 \\
0 & -1 & 1 & b_1 + b_2 \\
0 & 3 & -7 & b_1 + 3b_2 + b_3
\end{array}\right)
$$

#### (b) Multiply the Second Row by \(-1\).

$$
R_2 \to -R_2
$$

Resulting matrix:

$$
\left(\begin{array}{ccc|c}
1 & -2 & 3 & b_1 \\
0 & 1 & -1 & -(b_1 + b_2) \\
0 & 3 & -7 & b_1 + 3b_2 + b_3
\end{array}\right)
$$

#### (c) Add \(-3\) times the Second Row to the Third Row.

$$
R_3 \to R_3 - 3R_2
$$

Resulting matrix:

$$
\left(\begin{array}{ccc|c}
1 & -2 & 3 & b_1 \\
0 & 1 & -1 & -(b_1 + b_2) \\
0 & 0 & 0 & b_1 + 3b_2 + b_3
\end{array}\right)
$$

The third row gives the equation:

$$
b_1 + 3b_2 + b_3 = 0
$$

Thus, for the system to have a solution, the condition $b_1 + 3b_2 + b_3 = 0$ must hold. If this condition is satisfied, we can solve the system further.

### Solving for the Variables

Assume the values $b_1 = 2$, $b_2 = 1$, and $b_3 = -5$, so the condition is satisfied. The augmented matrix becomes:

$$
\left(\begin{array}{ccc|c}
1 & -2 & 3 & 2 \\
0 & 1 & -1 & -3 \\
0 & 0 & 0 & 0
\end{array}\right)
$$

We now have the system:

$$
x_1 - 2x_2 + 3x_3 = 2
$$

$$
x_2 - x_3 = -3
$$

### Step 1: Parametrize the Solution

Let $x_3 = \alpha$ (where $\alpha$ is arbitrary). Then from the second equation:

$$
x_2 = \alpha - 3
$$

Substitute $x_2 = \alpha - 3$ and $x_3 = \alpha$ into the first equation:

$$
x_1 - 2(\alpha - 3) + 3\alpha = 2
$$

$$
x_1 = -\alpha - 4
$$

Thus, the solution in vector form is:

$$
\mathbf{x} = \begin{pmatrix} -\alpha - 4 \\ \alpha - 3 \\ \alpha \end{pmatrix} = \alpha \begin{pmatrix} -1 \\ 1 \\ 1 \end{pmatrix} + \begin{pmatrix} -4 \\ -3 \\ 0 \end{pmatrix}
$$

Thus, the general solution to the system is:

$$
\mathbf{x} = \alpha \begin{pmatrix} -1 \\ 1 \\ 1 \end{pmatrix} + \begin{pmatrix} -4 \\ -3 \\ 0 \end{pmatrix}
$$

This shows the system has infinitely many solutions, where $\alpha$ is a free parameter.

## Linear Dependence and Independence of Vectors

### Definition

A set of vectors $\mathbf{x}(1), \mathbf{x}(2), \dots, \mathbf{x}(k)$ is **linearly dependent** if there exists a set of constants $c_1, c_2, \dots, c_k$, not all of which are zero, such that:

$$
c_1 \mathbf{x}(1) + c_2 \mathbf{x}(2) + \dots + c_k \mathbf{x}(k) = \mathbf{0}
$$

Otherwise, the set is **linearly independent**.

### Problem: Check if the Vectors Are Linearly Independent

Given the following vectors:

$$
\mathbf{x}^{(1)} = \begin{pmatrix} 1 \\ 2 \\ -1 \end{pmatrix}, \quad
\mathbf{x}^{(2)} = \begin{pmatrix} 2 \\ 1 \\ 3 \end{pmatrix}, \quad
\mathbf{x}^{(3)} = \begin{pmatrix} -4 \\ 1 \\ -11 \end{pmatrix}
$$

We want to check if these vectors are linearly independent by solving:

$$
c_1 \mathbf{x}^{(1)} + c_2 \mathbf{x}^{(2)} + c_3 \mathbf{x}^{(3)} = \mathbf{0}
$$

This gives the augmented matrix:

$$
\left(\begin{array}{ccc|c}
1 & 2 & -4 & 0 \\
2 & 1 & 1 & 0 \\
-1 & 3 & -11 & 0
\end{array}\right)
$$

### Step 1: Row Operations

#### (a) Subtract 2 times the First Row from the Second Row and Add the First Row to the Third Row.

$$
R_2 \to R_2 - 2R_1, \quad R_3 \to R_3 + R_1
$$

Resulting matrix:

$$
\left(\begin{array}{ccc|c}
1 & 2 & -4 & 0 \\
0 & -3 & 9 & 0 \\
0 & 5 & -15 & 0
\end{array}\right)
$$

#### (b) Divide the Second Row by \(-3\).

$$
R_2 \to \frac{1}{-3} R_2
$$

Resulting matrix:

$$
\left(\begin{array}{ccc|c}
1 & 2 & -4 & 0 \\
0 & 1 & -3 & 0 \\
0 & 5 & -15 & 0
\end{array}\right)
$$

#### (c) Subtract 5 times the Second Row from the Third Row.

$$
R_3 \to R_3 - 5R_2
$$

Resulting matrix:

$$
\left(\begin{array}{ccc|c}
1 & 2 & -4 & 0 \\
0 & 1 & -3 & 0 \\
0 & 0 & 0 & 0
\end{array}\right)
$$

This implies the system is dependent. The general solution is:

$$
c_1 \mathbf{x}^{(1)} + c_2 \mathbf{x}^{(2)} + c_3 \mathbf{x}^{(3)} = 0
$$

This equation simplifies to:

$$
2 \mathbf{x}^{(1)} - 3 \mathbf{x}^{(2)} - \mathbf{x}^{(3)} = 0
$$

Thus, the vectors are **linearly dependent**.

## Eigenvalues and Eigenvectors

Given the matrix:

$$
A = \begin{pmatrix} 3 & -1 \\ 4 & -2 \end{pmatrix}
$$

### Step 1: Characteristic Equation

We solve for the eigenvalues by computing the determinant of $ A - \lambda I $, where $I$ is the identity matrix:

$$
\det(A - \lambda I) = \det \begin{pmatrix} 3-\lambda & -1 \\ 4 & -2-\lambda \end{pmatrix} = (3-\lambda)(-2-\lambda) - (-4)
$$

Expanding the determinant:

$$
(3-\lambda)(-2-\lambda) + 4 = -6 - 3\lambda + 2\lambda + \lambda^2 + 4
$$

$$
= \lambda^2 - \lambda - 2
$$

Set this equal to zero:

$$
\lambda^2 - \lambda - 2 = 0
$$

Factor the quadratic equation:

$$
(\lambda - 2)(\lambda + 1) = 0
$$

Thus, the eigenvalues are:

$$
\lambda_1 = 2, \quad \lambda_2 = -1
$$

### Step 2: Eigenvectors

#### (a) For $\lambda_1 = 2$:

Solve $(A - 2I)\mathbf{x} = 0$:

$$
A - 2I = \begin{pmatrix} 1 & -1 \\ 4 & -4 \end{pmatrix}
$$

Solve the system:

$$
\mathbf{x} = \begin{pmatrix} 1 \\ 1 \end{pmatrix}
$$

#### (b) For $\lambda_2 = -1$:

Solve $(A + I)\mathbf{x} = 0$:

$$
A + I = \begin{pmatrix} 4 & -1 \\ 4 & -1 \end{pmatrix}
$$

Solve the system:

$$
\mathbf{x} = \begin{pmatrix} 1 \\ 4 \end{pmatrix}
$$

Thus, the eigenvectors corresponding to the eigenvalues $\lambda_1 = 2$ and $\lambda_2 = -1$ are:

$$
\mathbf{x}_1 = \begin{pmatrix} 1 \\ 1 \end{pmatrix}, \quad \mathbf{x}_2 = \begin{pmatrix} 1 \\ 4 \end{pmatrix}
$$
