---
tags:
  - mathematics/ordinary_differential_equations
---
# Homogenous Linear Systems with Constant Coefficients

Consider the system of first-order linear differential equations:

$$
x' = Ax, \tag{1}
$$

where $A$ is a constant coefficient matrix. Our objective is to solve such systems and analyze their behavior. We begin with a simple case.

## Example 1: Diagonal Matrix

Given the system:

$$
x' = 
\begin{pmatrix}
2 & 0 \\
0 & -3
\end{pmatrix}
x, \tag{2}
$$

we note that the coefficient matrix is diagonal. Writing the system in scalar form:

$$
x_1' = 2x_1, \quad x_2' = -3x_2.
$$

These equations are independent, and their solutions are:

$$
x_1 = c_1 e^{2t}, \quad x_2 = c_2 e^{-3t},
$$

where $c_1$ and $c_2$ are arbitrary constants. Rewriting the solution in vector form, we obtain:

$$
x = 
\begin{pmatrix}
x_1 \\
x_2
\end{pmatrix}
=
\begin{pmatrix}
c_1 e^{2t} \\
c_2 e^{-3t}
\end{pmatrix}
= c_1 
\begin{pmatrix}
1 \\
0
\end{pmatrix}
e^{2t} + c_2 
\begin{pmatrix}
0 \\
1
\end{pmatrix}
e^{-3t}. \tag{3}
$$

Defining the solutions:

$$
x^{(1)}(t) =
\begin{pmatrix}
1 \\
0
\end{pmatrix}
e^{2t}, \quad x^{(2)}(t) =
\begin{pmatrix}
0 \\
1
\end{pmatrix}
e^{-3t}, \tag{4}
$$

we compute the Wronskian:

$$
W[x^{(1)}, x^{(2)}](t) = 
\begin{vmatrix}
e^{2t} & 0 \\
0 & e^{-3t}
\end{vmatrix}
= e^{-t}. \tag{5}
$$

Since $W[x^{(1)}, x^{(2)}](t) \neq 0$, the solutions form a fundamental set, and the general solution is given by Eq. (3).

### General Case: Exponential Solutions and Eigenvalues

For the general system in Eq. (1), we propose solutions of the form:

$$
x = \xi e^{rt}, \tag{6}
$$

where $\xi$ is a constant vector, and $r$ is a scalar to be determined. Substituting Eq. (6) into Eq. (1) gives:

$$
r \xi e^{rt} = A \xi e^{rt}.
$$

Canceling the nonzero factor $e^{rt}$:

$$
(A - rI)\xi = 0, \tag{7}
$$

where $I$ is the identity matrix. Eq. (7) implies that $r$ is an eigenvalue of $A$, and $\xi$ is the associated eigenvector. Solving Eq. (1) reduces to determining the eigenvalues and eigenvectors of $A$.

## Example 2: 2 Ã— 2 System with Real Eigenvalues

Consider:

$$
x' = 
\begin{pmatrix}
1 & 1 \\
4 & 1
\end{pmatrix}
x. \tag{8}
$$

### Eigenvalue Computation

The eigenvalues satisfy:

$$
\det
\begin{pmatrix}
1 - r & 1 \\
4 & 1 - r
\end{pmatrix}
= (1 - r)^2 - 4 = r^2 - 2r - 3 = (r - 3)(r + 1) = 0. \tag{9}
$$

Thus, $r_1 = 3$ and $r_2 = -1$.

### Eigenvectors

For $r_1 = 3$:

$$
\begin{pmatrix}
-2 & 1 \\
4 & -2
\end{pmatrix}
\begin{pmatrix}
\xi_1 \\
\xi_2
\end{pmatrix}
= 
\begin{pmatrix}
0 \\
0
\end{pmatrix}.
$$

From $-2\xi_1 + \xi_2 = 0$, we find $\xi_2 = 2\xi_1$. Choosing $\xi_1 = 1$, the eigenvector is:

$$
\xi^{(1)} =
\begin{pmatrix}
1 \\
2
\end{pmatrix}. \tag{10}
$$

For $r_2 = -1$, a similar computation yields:

$$
\xi^{(2)} =
\begin{pmatrix}
1 \\
-2
\end{pmatrix}. \tag{11}
$$

### General Solution

The corresponding solutions are:

$$
x^{(1)}(t) =
\begin{pmatrix}
1 \\
2
\end{pmatrix}
e^{3t}, \quad x^{(2)}(t) =
\begin{pmatrix}
1 \\
-2
\end{pmatrix}
e^{-t}.
$$

The Wronskian is:

$$
W[x^{(1)}, x^{(2)}](t) =
\begin{vmatrix}
e^{3t} & e^{-t} \\
2e^{3t} & -2e^{-t}
\end{vmatrix}
= -4e^{2t}. \tag{12}
$$

The general solution is:

$$
x = c_1 x^{(1)}(t) + c_2 x^{(2)}(t) =
c_1 
\begin{pmatrix}
1 \\
2
\end{pmatrix}
e^{3t} + c_2 
\begin{pmatrix}
1 \\
-2
\end{pmatrix}
e^{-t}. \tag{13}
$$

## Example 3: Eigenvalues of the Same Sign

Consider:

$$
x' = 
\begin{pmatrix}
-3 & \sqrt{2} \\
\sqrt{2} & -2
\end{pmatrix}
x. \tag{14}
$$

### Eigenvalue Computation

The eigenvalues satisfy:

$$
\det
\begin{pmatrix}
-3 - r & \sqrt{2} \\
\sqrt{2} & -2 - r
\end{pmatrix}
= r^2 + 5r + 4 = (r + 1)(r + 4) = 0. \tag{15}
$$

Thus, $r_1 = -1$ and $r_2 = -4$.

### Eigenvectors

For $r_1 = -1$ and $r_2 = -4$, we find:

$$
\xi^{(1)} =
\begin{pmatrix}
1 \\
\sqrt{2}
\end{pmatrix}, \quad
\xi^{(2)} =
\begin{pmatrix}
-\sqrt{2} \\
1
\end{pmatrix}. \tag{16}
$$

### General Solution

The fundamental solutions are:

$$
x^{(1)}(t) =
\begin{pmatrix}
1 \\
\sqrt{2}
\end{pmatrix}
e^{-t}, \quad
x^{(2)}(t) =
\begin{pmatrix}
-\sqrt{2} \\
1
\end{pmatrix}
e^{-4t}.
$$

The general solution is:

$$
x = c_1 x^{(1)}(t) + c_2 x^{(2)}(t). \tag{17}
$$
